statecontext.bpl
@@ -1,0 +1,85 @@
+var myState: [Ref]Ref;
+
+var packedBasicFieldsContext : [Ref]bool;
+var fracBasicFieldsContext : [Ref]real;
+
+var packedStateContextMultiple2 : [Ref]bool;
+var fracStateContextMultiple2 : [Ref]real;
+
+var packedStateContextMultiple3 : [Ref]bool;
+var fracStateContextMultiple3 : [Ref]real;
+
+procedure PackStateContextMultiple2(m:Ref, this:Ref);
+requires (packedStateContextMultiple2[this] == false);
+requires (myState[this] == m);
+requires (instanceof[m] == 1) ==> (fracStateMultipleOf2StateLive[this] >= 1.0);
+requires (instanceof[m] == 2) ==> (fracStateMultipleOf2StateLimbo[this] >= 1.0);
+requires (instanceof[m] == 3) ==> (fracStateMultipleOf2StateSleep[this] >= 1.0);
+
+procedure UnpackStateContextMultiple2(m:Ref, this:Ref);
+requires packedStateContextMultiple2[this];
+ensures (myState[this] == m);
+ensures (instanceof[m] == 1) ==> (fracStateMultipleOf2StateLive[this] >= 1.0);
+ensures (instanceof[m] == 2) ==> (fracStateMultipleOf2StateLimbo[this] >= 1.0);
+ensures (instanceof[m] == 3) ==> (fracStateMultipleOf2StateSleep[this] >= 1.0);
+
+//	predicate BasicFieldsContext() = exists m:StateLike :: this.myState -> m
+
+//	predicate stateLive() = myState instanceof StateLive
+//	predicate stateSleep() = myState instanceof StateSleep
+//	predicate stateLimbo() = myState instanceof StateLimbo
+//	predicate stateContextMultiple2() = myState#1 StateMultipleOf2() 
+//	predicate stateContextMultiple3() = myState#1 StateMultipleOf3() 
+	
+StateContext() 
+ensures this#1 stateLive() 
+{ 
+	setState(new StateLive()); 
+} 
+
+void setState(Statelike newState) { 
+	myState = newState; 
+} 
+
+procedure computeResultSC(num: int) returns (r:Ref)
+modifies 
+ensures packedStateContextMultiple3[this];
+ensures fracStateContextMultiple3[this] >= 1.0;
+ensures (old(instanceof[mystate[this]]) == 1) ==> (instanceof[mystate[this]] == 2);
+ensures (old(instanceof[mystate[this]]) == 2) ==> (instanceof[mystate[this]] == 3);
+ensures (old(instanceof[mystate[this]]) == 3) ==> (instanceof[mystate[this]] == 1);
+{
+var temp : Ref;
+if (instanceof[myState[this]]) == 1) {
+	call temp := computeResultStateLive(this, num, myState[this]);
+} else if (instanceof[mystate[this]]) == 2) {
+	call temp := computeResultStateLimbo(this, num, myState[this]);
+} else {
+	call temp := computeResultStateSleep(this, num, myState[this]);
+}
+
+}
+
+public IntCell computeResult2SC(int num) 
+ensures (this#1 stateContextMultiple2())
+ensures (this#1.0 stateLive() ~=> (this#1.0 stateSleep())) 
+&& 
+(this#1.0 stateSleep() ~=> (this#1.0 stateLimbo())) 
+&&
+(this#1.0 stateLimbo() ~=> (this#1.0 stateLive()))
+{ 
+	return myState.computeResult2(this, num); 
+} 
+
+boolean stateContextCheckMultiplicity3() 
+requires this#1.0 stateContextMultiple3() 
+{ 
+	return myState.checkMod3(); 
+} 
+
+boolean stateContextCheckMultiplicity2() 
+requires this#1.0 stateContextMultiple2() 
+{ 
+	return myState.checkMod2(); 
+} 
+
